[1.6] partial completeness result

Logic/Chapter1/Section6.lean
@@ -1,10 +1,11 @@
 import Mathlib.Data.Set.Finite
 import «MathlibExt».Fin
 import «Logic».Chapter1.Section3
+import «Logic».Chapter1.Section4
 
 open Notation
 
-section Hilbert
+section Proof
 
 def Λ₁ : Set (Bₐ.Formula V) :=
   {(α ⟶ β ⟶ γ) ⟶ (α ⟶ β) ⟶ α ⟶ γ | (α : Bₐ.Formula V) (β : Bₐ.Formula V) (γ : Bₐ.Formula V)}
@@ -19,31 +20,45 @@ def Λ₃ : Set (Bₐ.Formula V) :=
 def Λ₄ : Set (Bₐ.Formula V) :=
   {(α ⟶ ~β) ⟶ β ⟶ ~α | (α : Bₐ.Formula V) (β : Bₐ.Formula V)}
 
-abbrev Λ : Set (Bₐ.Formula V) := Λ₁ ∪ Λ₂ ∪ Λ₃ ∪ Λ₄
-
-lemma mem_Λ {P : Bₐ.Formula V → Prop}
-    (h₁ : α ∈ Λ₁ → P α) (h₂ : α ∈ Λ₂ → P α) (h₃ : α ∈ Λ₃ → P α) (h₄ : α ∈ Λ₄ → P α)
-    (h : α ∈ Λ) : P α :=
-  Or.elim h (Or.elim · (Or.elim · h₁ h₂) h₃) h₄
-
-def is_proof (φs : [Bₐ.Formula V; n + 1]) (X : Set (Bₐ.Formula V)) :=
-    ∀ k, φs k ∈ X ∪ Λ ∨ ∃ i < k, ∃ j < k, φs j = φs i ⟶ φs k
+def Λ : Set (Bₐ.Formula V) := Λ₁ ∪ Λ₂ ∪ Λ₃ ∪ Λ₄
 
 /--
-  A proof of `α` from `X` of size `n + 1` is a sequence of formulas `φs` of length `n` such that
-  `φₙ = α` and for every `φₖ` in `φs` either
-  - `φₖ ∈ X ∪ Λ` (assumption)
+  A proof of `α` from `X` of size `n + 1` is a sequence of formulas `φs = [φ₀, .., φₙ]` of
+  length `n` such that `φₙ = α` and for every `φₖ` in `φs` either
+  - `φₖ ∈ X ∪ Λ` (assumption or tautology)
   - `∃ i < k, j < k, φⱼ = φᵢ → φₖ` (modus ponens)
 -/
 structure Proof (X : Set (Bₐ.Formula V)) (α : Bₐ.Formula V) (n : ℕ) where
   φs : [Bₐ.Formula V; (n + 1)]
-  valid : is_proof φs X
+  valid : ∀ k, φs k ∈ X ∪ Λ ∨ ∃ i < k, ∃ j < k, φs j = φs i ⟶ φs k
   conclusion : φs (Fin.last n) = α
 
-def Proof.size (_ : Proof X α n) : ℕ := n + 1
+namespace Proof
+
+example {p q : Bₐ.Formula V} : Proof {p, q} (p ⋏ q) 4 := by
+  refine' ⟨![p, q, p ⟶ q ⟶ p ⋏ q, q ⟶ p ⋏ q, p ⋏ q], fun k => _, rfl⟩
+  match k with
+  | 0 => exact Or.inl (Set.mem_union_left _ (Set.mem_insert _ _))
+  | 1 => exact Or.inl (Set.mem_union_left _  (Set.mem_insert_iff.mpr
+    (Or.inr (Set.mem_singleton_iff.mpr rfl))))
+  | 2 => exact Or.inl (Set.mem_union_right _ (Set.mem_union_left _
+    (Set.mem_union_left _ (Set.mem_union_right _ ⟨p, q, rfl⟩))))
+  | 3 => exact Or.inr ⟨0, Nat.le.step (Nat.le.step Nat.le.refl), 2, Nat.le.refl, rfl⟩
+  | 4 => exact Or.inr ⟨1, Nat.le.step (Nat.le.step Nat.le.refl), 3, Nat.le.refl, rfl⟩
+
+def size (_ : Proof X α n) : ℕ := n + 1
 
 /-- Any prefix of a proof `φs` is also a proof. -/
-def Proof.init (p : Proof X α n) (h : k < n) : Proof X (p.φs k) k := sorry
+def init (p : Proof X α n) (h : k < n) : Proof X (p.φs k) k := by
+  refine' ⟨Fin.init' p.φs (add_lt_add_right h 1), fun k' => _, _⟩
+  · refine' Or.elim (p.valid k') (fun hk' => Or.inl _) (fun ⟨i, hi, j, hj, hk'⟩ => Or.inr _)
+    · rw [Fin.init'_lt]
+      sorry
+    · sorry
+  · simp only [Fin.init', Fin.val_last]
+    rw [← (Fin.eq_mk_iff_val_eq (hk := h.trans (lt_add_one n))).mpr]
+    exact Fin.val_cast_of_lt (Nat.le.step h)
+
 -- def Proof.init (p : Proof X α n) (h : k < n) : Proof X (p.φs k) k := by
 --   refine' ⟨Fin.init' p.φs (add_lt_add_right h 1), _, _⟩
 --   · intro k'
@@ -72,29 +87,69 @@ def Proof.init (p : Proof X α n) (h : k < n) : Proof X (p.φs k) k := sorry
 --     rw [← (Fin.eq_mk_iff_val_eq (hk := h.trans (lt_add_one n))).mpr]
 --     exact Fin.val_cast_of_lt (Nat.le.step h)
 
+end Proof
+end Proof
+
 /-- A relation between sets of formulas and formulas. -/
-class Proves (α : Sort _) (β : Sort _) where
+class Hilbert (α : Sort _) (β : Sort _) where
   proves : α → β → Prop
 
-scoped[Notation] infix:40 " |~ " => Proves.proves
+scoped[Notation] infix:40 " |~ " => Hilbert.proves
 
-instance : Proves (Set (Bₐ.Formula V)) (Bₐ.Formula V) where
+instance : Hilbert (Set (Bₐ.Formula V)) (Bₐ.Formula V) where
   proves X α := ∃ n, Nonempty (Proof X α n)
 
-instance : Proves (Set (Bₐ.Formula V)) (Set (Bₐ.Formula V)) where
+instance : Hilbert (Set (Bₐ.Formula V)) (Set (Bₐ.Formula V)) where
   proves X Y := ∀ α ∈ Y, X |~ α
 
-example {p q : Bₐ.Formula V} : is_proof ![p, q, p ⟶ q ⟶ p ⋏ q, q ⟶ p ⋏ q, p ⋏ q] {p, q}
-  | 0 => Or.inl (Set.mem_union_left _ (Set.mem_insert _ _))
-  | 1 => Or.inl (Set.mem_union_left _  (Set.mem_insert_iff.mpr
-    (Or.inr (Set.mem_singleton_iff.mpr rfl))))
-  | 2 => Or.inl (Set.mem_union_right _ (Set.mem_union_left _
-    (Set.mem_union_left _ (Set.mem_union_right _ ⟨p, q, rfl⟩))))
-  | 3 => Or.inr ⟨0, Nat.le.step (Nat.le.step Nat.le.refl), 2, Nat.le.refl, rfl⟩
-  | 4 => Or.inr ⟨1, Nat.le.step (Nat.le.step Nat.le.refl), 3, Nat.le.refl, rfl⟩
+namespace Hilbert
 
-/-- Theorem 6.1: Induction principle for `|~`. -/
-theorem Hilbert.induction (P : Bₐ.Formula V → Prop) (ho : ∀ α ∈ X ∪ Λ, P α)
+section Lemmas
+
+variables {X X' : Set (Bₐ.Formula V)} {α β : Bₐ.Formula V}
+
+lemma singleton (α : Bₐ.Formula V) : ({α} : Set _) |~ α := by
+  refine' ⟨0, ⟨![α], fun k => Or.inl _, _⟩⟩
+  all_goals simp only [Matrix.cons_val_fin_one, Set.mem_union, Set.mem_singleton α, true_or]
+
+lemma mono (hX : X ⊆ X') (h : X |~ α) : X' |~ α := by
+  have ⟨n, ⟨p⟩⟩ := h
+  refine' ⟨n, ⟨p.φs, fun k => Or.elim (p.valid k)
+    (fun hk => Or.inl (Or.elim hk (fun hk => Or.inl (hX hk)) (fun hk => Or.inr hk)))
+    (fun hk => Or.inr hk),
+    p.conclusion⟩⟩
+
+lemma mp (hα : X |~ α) (hαβ : X |~ α ⟶ β) : X |~ β := by sorry
+  -- need to concat the proofs of α, α ⟶ β, and append β
+
+/-- Lemma 6.2.a. -/
+lemma contrapositive (h : X |~ α ⟶ ~β) : X |~ β ⟶ ~α := by sorry
+
+/-- Lemma 6.2.b. -/
+lemma assumption : (∅ : Set (Bₐ.Formula V)) |~ α ⟶ β ⟶ α := by sorry
+
+/-- Lemma 6.2.c. -/
+lemma identity : (∅ : Set (Bₐ.Formula V)) |~ α ⟶ α := by sorry
+
+/-- Lemma 6.2.d. -/
+lemma imp_not_not : (∅ : Set (Bₐ.Formula V)) |~ α ⟶ ~~α := by sorry
+
+/-- Lemma 6.2.e. -/
+lemma imp_not_imp_absurd : (∅ : Set (Bₐ.Formula V)) |~ β ⟶ ~β ⟶ α := by sorry
+
+/-- Lemma 6.3 (Deduction theorem). -/
+lemma deduction (h : X ∪ {a} |~ β) : X |~ α ⟶ β := by sorry
+
+/-- Lemma 6.4. -/
+lemma not_not_imp : (∅ : Set (Bₐ.Formula V)) |~ ~~α ⟶ α := by sorry
+
+/-- Lemma 6.5. -/
+lemma not₂ (h₁ : X ∪ {β} |~ α) (h₂ : X ∪ {~β} |~ α) : X |~ α := by sorry
+
+end Lemmas
+
+/-- Theorem 6.1: Induction principle for Hilbert Calculi `|~`. -/
+theorem induction (P : Bₐ.Formula V → Prop) (ho : ∀ α ∈ X ∪ Λ, P α)
     (hs : ∀ α β, P α → P (α ⟶ β) → P β) (hp : Proof X φ n) : P φ := by
   by_cases hφ : φ ∈ X ∪ Λ
   · exact ho φ hφ
@@ -116,6 +171,25 @@ termination_by _ => hp.size
 
 variable {X : Set (Bₐ.Formula V)} {α β : Bₐ.Formula V}
 
+/--
+  Finiteness of `|~`.
+
+  This can also be shown by identifying exactly which elements of `X` are used in the proof of `α`,
+  which will be finite since proofs are finite.
+-/
+theorem finiteness (h : X |~ α) : ∃ X₀ ⊆ X, X₀.Finite ∧ X₀ |~ α := by
+  have ⟨n, ⟨p⟩⟩ := h
+  refine' Hilbert.induction
+    (fun α => ∃ X₀ ⊆ X, X₀.Finite ∧ X₀ |~ α)
+    (fun α hα => Or.elim hα (fun hαX => ⟨{α}, _⟩) (fun hαΛ => _))
+    (fun α β ⟨Xα, hXαs, hXαf, hα⟩ ⟨Xβ, hXβs, hXβf, hβ⟩ => _)
+    p
+  · simp only [Set.singleton_subset_iff, Set.finite_singleton, hαX, true_and, singleton α]
+  · refine' ⟨{}, X.empty_subset, Set.finite_empty, ⟨0, ![α], fun k => Or.inl _, _⟩⟩
+    all_goals simp only [Matrix.cons_val_fin_one, Set.empty_union, hαΛ]
+  · refine' ⟨Xα ∪ Xβ, Set.union_subset_iff.mpr ⟨hXαs, hXβs⟩, Set.finite_union.mpr ⟨hXαf, hXβf⟩, _⟩
+    exact mp (mono (Xα.subset_union_left Xβ) hα) (mono (Xα.subset_union_right Xβ) hβ)
+
 /-- Soundness of `|~`. Equivalently, `|~ ⊆ ⊨`. -/
 theorem soundness (h : X |~ α) : X ⊨ α := by
   have ⟨n, ⟨p⟩⟩ := h
@@ -125,13 +199,8 @@ theorem soundness (h : X |~ α) : X ⊨ α := by
       (fun hαΛ w _ => _))
     (fun _ _ hα hαβ w hw => w.satisfies_arrow.mp (hαβ w hw) (hα w hw))
     p
-  · simp only [Set.mem_union] at hαΛ
-    refine' mem_Λ
-      (fun ⟨α, β, γ, h₁⟩ => _)
-      (fun ⟨α, β, h₂⟩ => _)
-      (fun h₃ => _)
-      (fun ⟨α, β, h₄⟩ => _)
-      hαΛ
+  · simp only [Set.mem_union, Λ, or_assoc] at hαΛ
+    obtain ⟨α, β, γ, h₁⟩ | ⟨α, β, h₂⟩ | h₃ | ⟨α, β, h₄⟩ := hαΛ
     · simp_rw [← h₁, Model.satisfies_arrow]
       exact fun hαβγ hαβ hα => hαβγ hα (hαβ hα)
     · simp_rw [← h₂, Model.satisfies_arrow]
@@ -143,9 +212,20 @@ theorem soundness (h : X |~ α) : X ⊨ α := by
       · rw [← h₃]
         simp only [Model.satisfies_arrow, Model.satisfies_and]
         exact fun ⟨_, hβ⟩ => hβ
-    · simp_rw [← h₄, Model.satisfies_arrow]
-      intro hαβ hβ
-      simp only [Model.satisfies_not]
-      exact fun hα => w.satisfies_not.mp (hαβ hα) hβ
+    · simp_rw [← h₄, Model.satisfies_arrow, Model.satisfies_not]
+      exact fun hαnβ hβ hα => hαnβ hα hβ
+
+/-- Theorem 6.6 (Completeness theorem). `|~ = ⊨`. -/
+theorem completeness [Inhabited V] : X |~ α ↔ X ⊨ α := by
+  refine' Iff.intro soundness (fun hXα => _)
+  refine' Gentzen.induction _ (Gentzen.completeness.mpr hXα)
+  constructor
+  · exact fun {α} => singleton α
+  · exact fun {X X' α} hX'α hXs => mono hXs hX'α
+  · sorry -- X |~ α → X |~ β → X |~ α ⋏ β
+  · sorry -- X |~ α ⋏ β → X |~ α
+  · sorry -- X |~ α ⋏ β → X |~ β
+  · sorry -- X |~ α → X |~ ~α → X |~ β
+  · exact fun {X α β} h₁ h₂ => not₂ h₁ h₂
 
 end Hilbert
